aneris/examples/reliable_communication/spec/api_spec.v
@@ -119,7 +119,7 @@ Section Init.
       Reliable_communication_init_setup
         E (UP : Reliable_communication_service_params):
       ↑RCParams_srv_N ⊆ E →
-      True ⊢ |={E}=>
+      ⊢ |={E}=>
         ∃ ( _ : Chan_mapsto_resource),
         ∃ (SnRes : SessionResources UP),
           SrvInit ∗
